Shallow water equations
=======================



<div id="fig:atmo">
![Layers of the atmosphere and the (source:
UCAR)](imgs/atmosphere_layers.jpg){#fig:atmo_layer width=60%}

![Annual zonal mean potential temperature - troposphere perspective (source:
ERA-40 atlas)](imgs/pot_temp_tropo_mean.eps){#fig:atmo_tropo width=45%}
![Annual zonal mean temperature - stratosphere perspective (source: ERA-40
atlas)](imgs/temp_strato_mean.eps){#fig:atmo_strat width=45%}

Stratification in atmosphere
</div>

The shallow-water equations are 

Governing Equations
-------------------

The governing equations for a shallow layer of fluid are:
\begin{align}
    \label{eq:dtu0} \partial_t \mathbf u & = - (\mathbf{u}.\nabla) \mathbf{u} - c^2 \nabla h - f\mathbf{e_z} \times \mathbf u \\
    \label{eq:dth} \partial_t h         & = - \nabla. (h \mathbf u)
\end{align}
Equation [@eq:dtu0] may also be written in the *rotational form* as:
$$\label{eq:dtu}
    \partial_t \mathbf u
    = - \nabla |\mathbf u|^2/2 - c^2 \nabla h - \zeta \times \mathbf u$$
where, [zeta]{acronym-label="zeta" acronym-form="singular+short"}
represents absolute vorticity, i.e. the sum of vorticity and system
rotation. Furthermore, equations [@eq:dtu0] and [@eq:dth] can be
combined to form an equation for the *total mass flux*,
[J]{acronym-label="J" acronym-form="singular+short"} $= h\mathbf{u}$:
$$\label{eq:dtJ}
    \partial_t \mathbf J = -(\mathbf{u}.\nabla)\mathbf{J} - \nabla(c^2h^2)/2 -
    \zeta \times \mathbf J - (\nabla. \mathbf J)\mathbf u$$ Similarly,
an equation for the *displaced mass flux*, [M]{acronym-label="M"
acronym-form="singular+short"} $=
    \eta\mathbf{u}$ is: $$\label{eq:dtM}
    \partial_t \mathbf M = -(\mathbf{u}.\nabla)\mathbf{M} - \nabla(c^2\eta^2)/2 -
    \zeta \times \mathbf M - (\nabla.\mathbf{u} + \nabla.\mathbf{M})\mathbf u$$
For a divergence free flow, a Poisson equation for *h* can be
formulated. Taking divergence of [@eq:dtu], yields the Poisson equation:
$$\label{eq:poisson}
    \nabla^2 h = \frac{1}{c^2} \left[ \nabla.(\zeta \times \mathbf u )
        - \nabla^2 \frac{|u|^2}{2} \right]$$ Applying fourier transform,
the spectral counterpart for [@eq:poisson] in tensor notation is:
$$\label{eq:poisson_fft}
    -\kappa^2 \hat{h} = \frac{1}{c^2} \left[ ik_i (\widehat{\epsilon_{ijk} \zeta_j
            u_k})
        + \kappa^2 \frac{\widehat{u_i u_i}}{2} \right]$$

Helmholtz Decomposition
-----------------------

### For velocity field, u

The Helmholtz decomposition theorem, or the fundamental theorem of
vector calculus, states that any well-behaved vector field can be
decomposed into the sum of a longitudinal (diverging, non-curling,
irrotational) vector field and a transverse (solenoidal, curling,
rotational, non-diverging) vector field. This allows us to express the
velocity field as:
\begin{align}
    \label{eq:helm_u}
    \mathbf u & = -\nabla \times (e_z \Psi) + \nabla \Phi \\
              & =  -\nabla \times \Psi_z + \nabla \Phi\end{align}

For the sake of clarity, we shall denote the rotational (vortical) and
divergent (wave) parts of the velocity with the suffix *r* and *d*
respectively. Thus,
\begin{align*}
    \mathbf u_r & = -\nabla \times \Psi_z ; & \mathbf u_d =   \nabla \Phi\end{align*}
 And therefore, $\mathbf u  = \mathbf u_r + \mathbf u_d$.

To find the projection operators for the divergent part, taking
divergence of [@eq:helm_u] gives $\nabla .\mathbf{u} = \nabla^2 \Phi$.
This transforms in the spectral plane as, $ik_j \hat{u}_j = -\kappa^2
    \hat{\Phi}$, implying:
\begin{align*}
    \mathbf{\hat{u}}_d = & ik_i \hat{\Phi} = \frac{k_i k_j}{\kappa^2} \hat{u}_j       \\
    \mathbf{\hat{u}}_r = & \mathbf{\hat{u}} - \mathbf{\hat{u}}_d = \left( \delta_{ij}
    - \frac{k_i k_j}{\kappa^2} \right) \hat{u}_j\end{align*}

Thus, for two-dimensions the decomposed velocity are represented as
follows,


\begin{align*}
    \mathbf{\hat{u}}_d^x = & \frac{k_x (k_x \hat{u}_x + k_y \hat{u}_y)}{\kappa^2}                \\
    \mathbf{\hat{u}}_r =   & \hat{u}_{x} - \frac{k_x  (k_x \hat{u}_x + k_y \hat{u}_y)}{\kappa^2}\end{align*}

### For fluid depth, h

To obtain a similar decomposition, $h = h_r + h_d$, one should use the
Poisson equation [@eq:poisson_fft]. Since Poisson equation requires a
divergence free flow, the LHS of [@eq:poisson_fft] would correspond to
the rotational part of the flow in the transformed plane, i.e.
$\hat{h}_r$. Henceforth, the divergent part, $\hat{h}_d$ can be obtained
by subtracting $\hat{h}_r$ from $\hat{h}$.

Normal mode decomposition
-------------------------

### Following Bartello 1995

In order to isolate oscillating fast modes that display no nonlinearity,
one can adopt a linearization approach followed by a normal mode
decomposition. As a result of linearization, from [@eq:dtu] and
[@eq:dth]:
\begin{align}
    \label{eq:dtu_l}
    \partial_t \mathbf u = & - c^2 \nabla \eta - f\mathbf{e_z} \times \mathbf u \\
    \label{eq:dth_l}
    \partial_t \eta =      & - \nabla.  \mathbf u\end{align}
 Taking curl and divergence of the linearized equation for momentum
[@eq:dtu_l] gives the following evolution equations with change of
variables:
\begin{align}
    \partial_t \zeta =  & - f \delta
    \label{eq:dtcurl_l}                                                  \\
    \partial_t \delta = & f \zeta - c^2 \nabla^2 \eta \label{eq:dtdiv_l} \\
    \partial_t \eta =   & - \delta \label{eq:dteta_l}\end{align}
 where $\zeta$ and $\delta$ are relative vorticity and divergence as
functions of $\mathbf{r}$ and $t$ respectively. Representing the
dependent flow quantities in terms of Fourier modes:
\begin{align*}
    \begin{pmatrix}
        u \\ v \\ \eta \\ \zeta \\ \delta
    \end{pmatrix} (\mathbf{r},t)
    = \int
    \begin{pmatrix}
        \hat{u} \\ \hat{v} \\ \hat{\eta} \\ \hat{\zeta} \\ \hat{\delta}
    \end{pmatrix} e^{i(\mathbf k . \mathbf{r} - \omega t)} \mathbf{dk} d\omega\end{align*}
 allows to rewrite the system of equations [@eq:dtcurl_l] to
[@eq:dteta_l] as an eigenvalue problem:
\begin{align*}
    i\omega
    \begin{Bmatrix}
        \hat{\zeta} \\ \hat{\delta} \\c\kappa\hat{\eta}
    \end{Bmatrix}
    = i
    \begin{bmatrix}
        0   & if       & 0         \\
        -if & 0        & -ic\kappa \\
        0   & ic\kappa & 0
    \end{bmatrix}
    \begin{Bmatrix}
        \hat{\zeta} \\ \hat{\delta} \\c\kappa\hat{\eta}
    \end{Bmatrix}\end{align*}
 where, $\kappa = |\mathbf{k}|$.

Let us define $A$ as the Hermitian matrix operating on the vector
$\mathbf{W} = \{\hat{\zeta}, \hat{\delta} ,c\kappa \hat{\eta} \}^T$.which
yields the familiar dispersion relation for the slow geostrophic mode
and fast Poincar√© wave modes:
$$\omega^{(0)} = 0;\quad \omega^{(\pm)}=\pm \sigma$$ where,
$\sigma = \sqrt{f^2 + c^2\kappa^2 }$. These are the eigenvalues of the
matrix operator *A*. Since *A* is Hermitian, the corresponding
eigenvectors are orthogonal and these are normalized as follows
\begin{align*}
    \mathbf X^{(0)}_n =
    \frac{1}{\sigma}
    \begin{Bmatrix}
        -c\kappa \\ 0 \\ f
    \end{Bmatrix}; \quad
    \mathbf X^{(\pm)}_n =
    \frac{1}{\sqrt{2} \sigma}
    \begin{Bmatrix}
        f \\ \mp i\sigma \\ c\kappa
    \end{Bmatrix}\end{align*}
 Let $X_n$ be the eigenvector matrix, which follows the property
$X_n \bar{X}_n^{T}=I$. It can, then, be applied to diagonalize the
system of equations as follows:
\begin{align*}
    \partial_t \mathbf{W} =               & [A] \mathbf{W}                    \\
    \partial_t (\bar{X}_n^T \mathbf{W}) = & \bar{X}_n^T[A]X_n
    \bar{X}_n^T\mathbf{W}                                                     \\
    =                                     & [\Lambda] (\bar{X}_n^T\mathbf{W})\end{align*}
 Thus, the alternate diagonalized system of equations for the normal
modes are given by:
\begin{align*}
    \partial_t
    \mathbf{N}
    = &
    \begin{bmatrix}
        0 & 0        & 0       \\
        0 & -i\sigma & 0       \\
        0 & 0        & i\sigma
    \end{bmatrix}
    \mathbf{N}                   \\
    \text{where},
    \mathbf{N} = \bar{X}_n^T \mathbf{W}
    = & \frac{1}{\sqrt{2}\sigma}
    \begin{Bmatrix}
        -\sqrt{2}c\kappa(\hat{\zeta} -f \hat{\eta})                \\
        f\hat{\zeta} + c^2\kappa^2\hat{\eta} - i\sigma\hat{\delta} \\
        f\hat{\zeta} + c^2\kappa^2\hat{\eta} + i\sigma\hat{\delta}
    \end{Bmatrix}\end{align*}

The first mode represents *linearised potential vorticity* which is
conserved in this framework. The remaining two are the *linearised
ageostrophic or wave modes*. In the absence of system rotation, i.e.
$f=0$, the normal modes are simply, $$\label{eq:nmode}
    \mathbf{N} =
    \begin{Bmatrix}
        \hat \zeta                                              \\
        \frac{1}{\sqrt{2}} (c\kappa \hat{\eta} - i\hat{\delta}) \\
        \frac{1}{\sqrt{2}} (c\kappa \hat{\eta} + i\hat{\delta})
    \end{Bmatrix}$$

### Following Farge & Sadourny 1989

Instead of finding the normal modes for the vorticity, divergence and
displacement field of the flow, we shall make use of the Helmholtz
decomposition described in [@eq:helm_u]. The shallow water equations
then transform to:
\begin{align}
    \partial_t \psi = & f \phi
    \label{eq:dtpsi_l}                                        \\
    \partial_t \phi = & -f \psi - c^2 \eta \label{eq:dtphi_l} \\
    \partial_t \eta = & - \nabla^2 \phi \label{eq:dteta_l2}\end{align}
 where $\psi$ and $\psi$ are stream function and velocity potential as
functions of $\mathbf{r}$ and $t$ respectively. By substituting the
dependent variables with the respective Fourier transform, this reduces
to the eigenvalue problem:
\begin{align*}
    i\omega
    \begin{Bmatrix}
        \hat{\psi} \\ \hat{\phi} \\ \hat{\eta}
    \end{Bmatrix}
    = i
    \begin{bmatrix}
        0   & if         & 0    \\
        -if & 0          & ic^2 \\
        0   & -i\kappa^2 & 0
    \end{bmatrix}
    \begin{Bmatrix}
        \hat{\psi} \\ \hat{\phi} \\ \hat{\eta}
    \end{Bmatrix}\end{align*}
 the square matrix is not Hermitian and this would result in complex
eigenvalues. By adopting the following change of variables:
$$\hat{\psi} \to \kappa^2\hat \psi = \hat{\zeta} ; \quad
    \hat{\phi} \to -\kappa^2\hat \phi = \hat{\delta}; \quad
    \hat{\eta} \to c\kappa\hat \eta$$ it falls back to the previous
eigenvalue problem as demonstrated in the previous section. In other
words, we can use the same eigenvector matrix, $X_n$ to find the normal
modes of:

$$\mathbf{H} = \{\hat \psi,\; \hat \phi,\;  \eta  \}^T$$ which is
closely related to: $$\mathbf{W}
    = \{\kappa^2\hat \psi,\; -\kappa^2\hat
    \phi,\; c\kappa\hat \eta  \}^T
    = \{\hat \zeta;\; \hat \delta;\;  c\kappa \hat \eta \}^T$$

### Normal mode inversion to primitive variables

To begin with, we shall form a new vector
$\mathbf{B} = \mathbf{N}/\kappa$ which will have the same dimensions as
velocity. It has been shown before that the normal modes can be
represented by $\mathbf{N}
    = \bar{X}_n^T \mathbf{W}$. Now, we shall form a new vector
$\mathbf{B} =
    \mathbf{N}/\kappa$ which will have the same dimensions as velocity.
Thus,
\begin{align*}
    \mathbf{B}
    = & \frac{1}{\sqrt{2}\sigma}
    \begin{Bmatrix} \sqrt{2} c\left(-
        \kappa^{2} \hat \psi +  f\hat\eta \right)               \\
        \kappa \left(c^{2} \eta + f \psi + i \phi \sigma\right) \\
        \kappa \left(c^{2} \eta + f \psi - i \phi \sigma\right)
    \end{Bmatrix}\end{align*}

The $\mathbf{B}$ vector can also be related to the primitive variable
vector, $\mathbf{U} = \{\hat{u},\hat{v},c\hat{\eta}\}^T$ using
transformation matrices as follows:
\begin{align*}
    \mathbf{B} = & \frac{1}{\kappa}[\bar{X}_n]^T W              \\
    =            & \frac{1}{\kappa}[\bar{X}_n]^T [P] \mathbf{U}\end{align*}
 where, $$P=
    \begin{bmatrix}- i k_{y} & i k_{x} & 0 \\ i k_{x} &  i
        k_{y}     &
        0                       \\0 & 0 & \kappa\end{bmatrix}$$ It is
also straightforward to show that the magnitude of the normal modes
equals the total energy as:
\begin{align*}
    \mathbf{\bar B}^T\mathbf{B}
    = & \frac{1}{\kappa^2} \mathbf{\bar U}^T
    [\bar P]^T[{X}_n]  [\bar{X}_n]^T [P] \mathbf{U} \\
    = & \mathbf{\bar U}^T\mathbf{U}\end{align*}
 implying, $$2(E_K+E_P)=\sum_i B^{(i)}\bar{B}^{(i)}=\kappa^{2} \psi
    \overline{\psi} +\kappa^{2} \phi \overline{\phi} + c^{2}
    \eta \overline{\eta}
    = u\bar{u} + v\bar{v} + c^2\eta\bar{\eta}$$ This allows us to
represent the primitive variables in terms of normal modes as
$$\mathbf{U} = [Q]\mathbf{B}$$ where, the inversion matrix is
\begin{align*}
    Q
    = & \kappa [P]^{-1}[\bar{X}_n]^{T^{-1}} \\
    = & \frac{1}{\sqrt{2}\sigma\kappa}
    \begin{bmatrix}
        -i\sqrt{2}c\kappa  k_{y}                    &
        \left(i f k_{y} +
        k_{x}   \sigma\right)                       &
        \left(i f k_{y} - k_{x} \sigma\right)         \\
        i \sqrt{2}c\kappa k_{x}                     &
        \left(-  i f k_{x} +  k_{y}   \sigma\right) &
        - \left(i f  k_{x} + k_{y} \sigma\right)      \\
        \sqrt{2}\kappa f                            &
        c\kappa^{2}                                 &
        c\kappa^{2}
    \end{bmatrix}\end{align*}
 In tensor notation,
\begin{align*}
    \hat{u}_l =   & \epsilon_{lm3} ik_m\left[ -\frac{c}{\sigma} B^{(0)} +
        \frac{f}{\sqrt{2}\sigma\kappa} (B^{(+)} + B^{(-)})
        \right]
    + k_l \frac{1}{\sqrt{2}\kappa}  (B^{(+)} - B^{(-)})                       \\
    c\hat{\eta} = & \frac{f}{\sigma} B^{(0)} + \frac{c\kappa}{\sqrt{2}\sigma}
    (B^{(+)} + B^{(-)})\end{align*}

Spectral energy budget
----------------------

### Kinetic energy

Kinetic energy being cubic for shallow water equations, it can be split
into quadratic and non-quadratic parts as follows:
\begin{align*}
    E_K(\mathbf{r},t)
    = & h\mathbf{u}.\mathbf{u}                            \\
    = & (1+\eta)\mathbf{u}.\mathbf{u}                     \\
    = & \mathbf{u}.\mathbf{u} + \eta\mathbf{u}.\mathbf{u} \\
    = & E_K^Q + E_K^{NQ}\end{align*}

Let the rate of change of kinetic energy, without any approximations, be
written as: $$\label{eq:dtKE}
    \pder{t}E_K(\mathbf{k},t) = T_K + C_K$$ where, $T_K$ and $C_K$
represents the transfer and conversion spectral functions respectively.
Equation [@eq:dtKE] splits into:
\begin{align*}
    \pder{t}E_K^Q + \pder{t}E_K^{NQ}
    = & (T_K^{Q} + C_K^{Q}) + (T_K^{NQ} + C_K^{NQ})\end{align*}

#### Quadratic K.E. budget:

Consider the rate of change of quadratic kinetic energy,
$$\label{eq:dtKE2}
    \pder{t}E_K^{Q}(\mathbf{k},t) = T_K^{Q} + C_K^{Q}$$ Following
[@eq:dtu0], equation [@eq:dtKE2] expands into:
\begin{align*}
    \partial_t E_K^{Q}(\mathbf{k},t)
    = & \frac{1}{2}\partial_t(\mathbf{\hat u}.\mathbf{\hat u^*})       \\
    = & \frac{1}{2}\left[ \mathbf{\hat u} .\pder[\mathbf{\hat u^*}]{t}
        + \mathbf{\hat u^*}. \pder[\mathbf{\hat u}]{t}\right]          \\
    = & \frac{1}{2}\left[ -\hat{u}_i (\widehat{ u_j\partial_j u_i })^*
        - c^2 \hat{u}_i (ik_i \hat{\eta})^*
        - \hat{u}_i (\epsilon_{i3k} f \hat{u}_k)^*
        - ... \text{conjugate terms}
        \right]                                                        \\
    = & -\text{Re}\left[ \hat{u}_i (\widehat{ u_j\partial_j u_i })^*
        + c^2 \hat{u}_i (ik_i \hat{\eta})^*
        + \hat{u}_i (\epsilon_{i3k} f \hat{u}_k)^* \right]\end{align*}
 we have,
\begin{align*}
    T_K^{Q}= & -\text{Re}\left[\hat{u}_i (\widehat{ u_j\partial_j u_i })^*
        \right]                                                              \\
    C_K^{Q}= & -\text{Re}\left[   c^2 \hat{u}_i (ik_i \hat{\eta})^*  \right] \\
    =        & -\text{Re}\left[   c^2 \hat{u}_i^* ik_i \hat{\eta} \right]\end{align*}

#### Non-quadratic K.E. budget:


\begin{align*}
    \pder{t}E_K^{NQ}(\mathbf{k},t) = & T_K^{NQ} + C_K^{NQ}\end{align*}
 Following equations [@eq:dtu0] and [@eq:dtM] for rate of change of
velocity $\mathbf{u}$ and the displaced mass flux,
$\mathbf M = \eta \mathbf{u}$ respectively,
\begin{align*}
    \partial_t E_K^{NQ}(\mathbf{k},t)
    = & \frac{1}{2}\partial_t(\mathbf{\hat M}.\mathbf{\hat u^*})        \\
    = & \frac{1}{2}\left[ \mathbf{\hat M} .\pder[\mathbf{\hat u^*}]{t}
        + \mathbf{\hat u^*}. \pder[\mathbf{\hat M}]{t}\right]           \\
    = & \frac{1}{2}\left[-\hat{M}_i(\widehat{ u_j\partial_j u_i })^*
        - c^2 \hat{M}_i (ik_i \hat{\eta})^*
        - \hat{M}_i (\epsilon_{i3k} f \hat{u}_k)^* \right]              \\
      & +\frac{1}{2}\left[ - \hat{u}_i^* \widehat{(u_j\partial_j M_i) }
        - c^2\hat{u}_i^*ik_i\widehat{\eta\eta}/2
        - \hat{u}_i^* (\epsilon_{i3k} f \hat{M}_k)
        - \hat{u_i}^* \widehat{(u_i \partial_j({u}_j+
            M_j))}
        \right]\end{align*}
 Hence,
\begin{align*}
    T_K^{NQ}=       & -\frac{1}{2}\left[\hat{M}_i(\widehat{ u_j\partial_j u_i })^*
        + \hat{u}_i^* \widehat{(u_j\partial_j M_i) }
        + \hat{u_i}^* \widehat{(u_i \partial_j{M}_j)}
        \right]                                                                    \\
    T_{K,K}^{NQ,Q}= & -\frac{1}{2}\left[ \hat{u_i}^* \widehat{(u_i
            \partial_j{u}_j)}
        \right]                                                                    \\
    T_{K,P}^{NQ,Q}= & -\frac{1}{2}\left[c^2 \hat{M}_i (ik_i \hat{\eta})^*
        + c^2\hat{u}_i^*ik_i\widehat{\eta\eta} /2
        \right]\end{align*}

Furthermore, using Helmholtz decomposition to substitute for $\mathbf u$
in the expression for *mean kinetic energy*,


\begin{align*}
    \braket{ E_K}
     & = \frac{1}{2} \braket{ h\mathbf u.\mathbf u}                          \\
     & = \frac{1}{2} \braket{h(\mathbf{u_r} + \mathbf{u_d} ).(\mathbf{u_r} +
        \mathbf{u_d} )}                                                      \\
     & = \frac{1}{2}\braket{ h |\mathbf{u_r} | ^2}
    -\braket{ \mathbf{u_r}.h\mathbf{u_d}}
    +  \frac{1}{2} \braket{ h | \mathbf{u_d}| ^2}\end{align*}
 where, $h = 1 + \eta$ and, $\eta$ is the surface displacement of the
shallow water layer. In the limit for small displacements i.e.,
$\eta \to 0$ or $h \to
    1$, invoking orthogonality,

$$\lim_{h \to 1} \braket{E_K} = \braket{E_K^{Q}}
    =  \frac{1}{2}\braket{|\mathbf{u_r}  | ^2 + | \mathbf{u_d} | ^2}$$
The spectral equivalent of the above expression will be:
$$\braket{E_K^{Q} }
    =  \frac{1}{2}\braket{ \mathbf{\hat{u}_r}.\mathbf{\hat{u}_r}^* +
        \mathbf{\hat{u}_d}.\mathbf{\hat{u}_d}^* }$$

### Available potential energy


\begin{align*}
    \braket{ E_P}
     & = \frac{c^2}{2} \braket{ \eta^2}\end{align*}
 The spectral equivalent of which is:
\begin{align*}
    \braket{ E_P}
     & = \frac{c^2}{2} \braket{ \hat{\eta}\hat{\eta}^*}\end{align*}

Similar to equation [@eq:dtKE] we can form, $$\label{eq:dtPE}
    \pder{t}E_P(\mathbf{k},t) = T_P+ C_P$$ where, $T_P$ and $C_P$
represents the transfer and conversion spectral functions respectively.

Following [@eq:dth], equation [@eq:dtPE] expands as:
\begin{align*}
    \pder{t}E_P(\mathbf{k},t)
    = & \frac{c^2}{2}\partial_t({\hat \eta}{\hat \eta^*})                 \\
    = & \frac{c^2}{2}\left[ \hat{\eta} .\pder[\hat{\eta}^*]{t}+ \hat
        \eta^*.\pder[\hat \eta]{t}\right]                                 \\
    = & \frac{c^2}{2}\left[ - \hat{\eta} (ik_i\hat{ u_i } + ik_i\widehat{
            \eta u_i })^*
        - \hat{\eta}^* (ik_i\hat{ u_i } + ik_i\widehat{
            \eta u_i })  \right]                                          \\
    = & -\text{Re}\left[c^2\hat{\eta} (ik_i\hat{ u_i } + ik_i\widehat{
            \eta u_i })^* \right]\end{align*}
 Thus,
\begin{align*}
    T_P= & -\text{Re}\left[c^2\hat{\eta} (ik_i\widehat{
            \eta u_i })^*  \right]                                 \\
    C_P= & -\text{Re}\left[c^2\hat{\eta} (ik_i\hat{u_i })^*\right] \\
    =    & +\text{Re}\left[c^2\hat{\eta} ik_i\hat{u_i }^*\right]\end{align*}
 thus, $C^Q_K = -C_P$ which, in turn, makes the assertion that
equivalent conversion occurs between quadratic K.E. and A.P.E.
